Tluh (#295)
* Issue 291: Started drafting the TlLink converter functions.

* Issue 291: UNSTABLE.

* Issue 291: UNSTABLE.

* Issue 291: Drafted TileLink message adaptors.

* Issue 291: reviewed, corrected, and filled in memOpNameToOpcode and memOpNameToParam.

* Issue 291: Removed TlFull from FU. Moved memOpCodeToMask back to TlUh.v. Marked several functions as local. Rewrote the check that confirms that the memory op codes are sufficiently wide to support all of the memory operations listed in MemOps.v. Removed calls to ZeroExtendTruncLsb from TlUh.v where appropriate.

Instance.v
@@ -7,6 +7,7 @@
 Require Import Kami.All Kami.Compiler.Compiler Kami.Compiler.Rtl Kami.Compiler.UnverifiedIncompleteCompiler.
 Require Import ProcKami.FU.
 Require Import ProcKami.Pipeline.ProcessorCore.
+Require Import ProcKami.MemOps.
 Require Import List.
 Import ListNotations.
 Require Import ProcKami.ModelParams.
@@ -53,11 +54,33 @@ Definition model (xlens : list nat) : Mod
        debug_buffer_sz
        debug_impebreak.
 
+Definition modelParams (xlens : list nat) : ProcParams
+  := modelProcParams
+       xlens
+       supportedExts
+       allow_misaligned
+       allow_inst_misaligned
+       misaligned_access 
+       (_ 'h"1000")
+       debug_buffer_sz
+       debug_impebreak.
+
 Definition xlens32 := [Xlen32].
 Definition xlens64 := [Xlen32; Xlen64].
 
 Definition model32 : Mod := model [Xlen32].
 Definition model64 : Mod := model [Xlen32; Xlen64].
+
+Definition model32Params := modelParams xlens32.
+Definition model64Params := modelParams xlens64.
+
+(* verify that the 32 bit model is compatible with TileLink. *)
+Goal Nat.log2_up (length (@memOps model32Params)) <= (@TlFullSz model32Params).
+Proof. cbv; lia. Qed.
+
+(* verify that the 64 bit model is compatible with TileLink. *)
+Goal Nat.log2_up (length (@memOps model64Params)) <= (@TlFullSz model64Params).
+Proof. cbv; lia. Qed.
 
 (** vm_compute should take ~40s *)
 
@@ -73,21 +96,10 @@ Proof.
   reflexivity.
 Qed.
 
-Definition procParams (xlens : list nat) : ProcParams
-  := ModelParams.procParams
-       xlens
-       supportedExts
-       allow_misaligned
-       allow_inst_misaligned
-       misaligned_access
-       (_ 'h"1000")
-       debug_buffer_sz
-       debug_impebreak.
-
 Definition meths (xlens : list nat) := [
   ("proc_core_ext_interrupt_pending", (Bit 0, Bool));
   ("proc_core_readUART", (UartRead, Data));
-  ("proc_core_writeUART", (@UartWrite (procParams xlens), Bit 0))
+  ("proc_core_writeUART", (@UartWrite (modelParams xlens), Bit 0))
 ].
 
 Axiom cheat : forall {X},X.
