TlUH.v
@@ -1,0 +1,135 @@
+Require Import Kami.AllNotations.
+Require Import ProcKami.FU.
+Require Import ProcKami.Device.
+Require Import ProcKami.MemOps.
+Require Import ProcKami.MemOpsFuncs.
+
+Section tluh.
+  Context {procParams : ProcParams}.
+
+  Section tlLink.
+    Context (tagK : Kind).
+
+    Definition ChannelAReq := STRUCT_TYPE {
+      "a_opcode"  :: TlOpcode;
+      "a_param"   :: TlParam;
+      "a_size"    :: TlSize;
+      "a_source"  :: Bit (size tagK);
+      "a_address" :: PAddr;
+      "a_mask"    :: Bit (size DataMask);
+      "a_corrupt" :: Bool;
+      "a_data"    :: Data
+    }.
+
+    (* Note: opcode is always Ack, param is always 0, and size is always the encoding of Rlen. *)
+    Definition ChannelDRes := STRUCT_TYPE {
+      "d_opcode"  :: TlOpcode;
+      "d_param"   :: TlParam;
+      "d_size"    :: TlSize;
+      "d_source"  :: Bit (size tagK);
+      "d_sink"    :: Void;
+      "d_denied"  :: Bool;
+      "d_corrupt" :: Bool;
+      "d_data"    :: Data
+    }.
+
+    Section ty.
+      Variable ty : Kind -> Type.
+
+      Local Open Scope kami_expr.
+
+      (*
+        TODO: determine if TileLink uses the mask as a bytle level
+        data mask and determine if this information is redundant
+        w.r.t the size and address params. *)
+      Local Definition memOpCodeToMaskAux
+        (sz : TlSize @# ty)
+        :  Bit (size DataMask) @# ty
+        := pack
+             ((utila_find_pkt
+               (map
+                 (fun n : nat
+                   => STRUCT {
+                        "valid" ::= (sz == $n);
+                        "data"  ::= getMask n ty
+                      } : Maybe DataMask @# ty)
+                 (seq 0 (Nat.pow 2 TlSizeSz)))) @% "data").
+
+      Local Definition memOpCodeToMask
+        (code : MemOpCode @# ty)
+        (address : PAddr @# ty)
+        :  Bit (size DataMask) @# ty
+        := let size := ZeroExtendTruncLsb TlSizeSz code in
+           let which : Bit 3 @# ty := (ZeroExtendTruncLsb 3 address) >> size in
+           ((memOpCodeToMaskAux size) << which).
+
+      Definition fromKamiReq
+        (req : Device.Req tagK @# ty)
+        :  ChannelAReq @# ty
+        := STRUCT {
+             "a_opcode"  ::= UniBit (TruncMsb _ TlOpcodeSz) (req @% "memOp");
+             "a_param"
+               ::= UniBit (TruncMsb (0 + TlSizeSz) TlParamSz)
+                     (UniBit (TruncLsb (0 + TlSizeSz + TlParamSz) TlOpcodeSz)
+                       (req @% "memOp"));
+             "a_size"
+               ::= UniBit (TruncLsb (0 + TlSizeSz) TlParamSz)
+                     (UniBit (TruncLsb (0 + TlSizeSz + TlParamSz) TlOpcodeSz)
+                       (req @% "memOp"));
+             "a_source"  ::= pack (req @% "tag");
+             "a_address" ::= (req @% "offset");
+             "a_mask"    ::= memOpCodeToMask (req @% "memOp") (req @% "offset");
+             "a_corrupt" ::= $$false;
+             "a_data"    ::= req @% "data"
+           }.
+
+      Definition toKamiReq
+        (req : ChannelAReq @# ty)
+        :  Device.Req tagK @# ty
+        := STRUCT {
+             "tag"    ::= unpack tagK (req @% "a_source");
+             "memOp"
+               ::= 
+                     ({< req @% "a_opcode", req @% "a_param", req @% "a_size" >});
+             "offset" ::= req @% "a_address";
+             "data"   ::= req @% "a_data"
+           }.
+
+      (*
+        NOTE: Murali instructed me to set d_denied and d_corrupt
+        so that they always indicate that the message is valid.
+      *)
+      Definition fromKamiRes
+        (res : Device.Res tagK @# ty)
+        :  ChannelDRes @# ty
+        := STRUCT {
+             "d_opcode"  ::= $TlAccessAckData;
+             "d_param"   ::= $0;
+             "d_size"    ::= $Rlen;
+             "d_source"  ::= pack (res @% "tag");
+             "d_sink"    ::= $$(getDefaultConst Void);
+             "d_denied"  ::= $$false;
+             "d_corrupt" ::= $$false;
+             "d_data"    ::= res @% "res" @% "data"
+           }.
+
+      (*
+        NOTE: Murali instructed me to set valid so that it always
+        indicate that the message is valid.
+      *)
+      Definition toKamiRes
+        (res : ChannelDRes @# ty)
+        :  Device.Res tagK @# ty
+        := STRUCT {
+             "tag" ::= unpack tagK (res @% "d_source");
+             "res"
+               ::= STRUCT {
+                     "valid" ::= $$true;
+                     "data"  ::= res @% "d_data"
+                   }
+           }.
+
+      Local Close Scope kami_expr.
+    End ty.  
+  End tlLink.
+End tluh.
